src/program_proof/examples/assumptions.v
@@ -5,18 +5,26 @@ From Perennial.program_proof Require Import proof_prelude.
 From Perennial.program_proof.examples Require Import
      replicated_block_proof single_inode_proof dir_proof.
 
+Goal True.
+idtac "replicated block:".
 Print Assumptions replicated_block_proof.init_zero_cinv. (* not used by [OpenRead] *)
 Print Assumptions replicated_block_proof.OpenRead_adequate.
 
-(* FIXME: also prove and check zero_init lemma. *)
+idtac "".
+idtac "single inode initialization:".
 Print Assumptions single_inode_proof.wpc_Open.
 Print Assumptions single_inode_proof.is_single_inode_alloc.
 Print Assumptions single_inode_proof.init_single_inode.
+idtac "single inode operations".
 Print Assumptions single_inode_proof.wpc_Read.
 Print Assumptions single_inode_proof.wpc_Append.
 
+idtac "".
+idtac "directory initialization:".
 Print Assumptions dir_proof.wpc_Open.
 Print Assumptions dir_proof.is_dir_alloc.
 Print Assumptions dir_proof.init_dir.
+idtac "directory operations:".
 Print Assumptions dir_proof.wpc_Read.
 Print Assumptions dir_proof.wpc_Append.
+Abort.
